[minor] [verif] SFI concrete properties.

sfi/symbolic.v
@@ -4,7 +4,8 @@ Require Import ssreflect ssrfun ssrbool eqtype ssrnat seq.
 
 Require Import lib.utils lib.ordered lib.partial_maps common.common.
 Require Import symbolic.symbolic symbolic.rules.
-Require Import sfi.classes sfi.list_utils sfi.set_utils sfi.isolate_sets.
+Require Import sfi.classes sfi.list_utils sfi.set_utils sfi.isolate_sets
+               sfi.ranges.
 
 Set Bullet Behavior "Strict Subproofs".
 
@@ -85,10 +86,12 @@ Qed.
 Definition stag_eqMixin := EqMixin stag_eqP.
 Canonical stag_eqType := Eval hnf in EqType stag stag_eqMixin.
 
-Context {memory : Type}
-        {sm : partial_map memory (word t) (atom (word t) stag)}
+Context {memory    : Type}
+        {sm        : partial_map memory (word t) (atom (word t) stag)}
+        {sma       : axioms sm}
         {registers : Type}
-        {sr : partial_map registers (reg t) (atom (word t) stag)}.
+        {sr        : partial_map registers (reg t) (atom (word t) stag)}
+        {sra       : axioms sr}.
 
 Import DoNotation.
 
@@ -119,26 +122,27 @@ Definition rvec_next : stag -> stag -> option (RVec stag) :=
   rvec_simple INTERNAL.
 Definition rvec_jump : stag -> stag -> option (RVec stag) :=
   rvec_simple JUMPED.
-Definition rvec_store (c' : word t) (W : list (word t))
+Definition rvec_store (c : word t) (I W : list (word t))
                       : stag -> stag -> option (RVec stag) :=
-  rvec_step (fun c =>
-    do! guard (c == c') || set_elem c W;
-    Some (sfi_rvec INTERNAL c)).
+  rvec_step (fun c' =>
+    do! guard (c == c') || set_elem c' W;
+    Some (mkRVec (PC INTERNAL c') (DATA c I W))).
 
 (* The `REG's in the MVec's fields can also be _s; it's an invariant that
    registers are always tagged with `REG'. *)
 Definition sfi_handler (mv : MVec stag) : option (RVec stag) :=
   match mv with
-    | mkMVec NOP       Lpc LI []                      => rvec_next       Lpc LI
-    | mkMVec CONST     Lpc LI [REG]                   => rvec_next       Lpc LI
-    | mkMVec MOV       Lpc LI [REG; REG]              => rvec_next       Lpc LI
-    | mkMVec (BINOP _) Lpc LI [REG; REG; REG]         => rvec_next       Lpc LI
-    | mkMVec LOAD      Lpc LI [REG; DATA _ _ _; REG]  => rvec_next       Lpc LI
-    | mkMVec STORE     Lpc LI [REG; REG; DATA c' _ W] => rvec_store c' W Lpc LI
-    | mkMVec JUMP      Lpc LI [REG]                   => rvec_jump       Lpc LI
-    | mkMVec BNZ       Lpc LI [REG]                   => rvec_next       Lpc LI
-    | mkMVec JAL       Lpc LI [REG; REG]              => rvec_jump       Lpc LI
-    | mkMVec _         _   _  _                       => None
+    | mkMVec NOP       Lpc LI []                     => rvec_next        Lpc LI
+    | mkMVec CONST     Lpc LI [REG]                  => rvec_next        Lpc LI
+    | mkMVec MOV       Lpc LI [REG; REG]             => rvec_next        Lpc LI
+    | mkMVec (BINOP _) Lpc LI [REG; REG; REG]        => rvec_next        Lpc LI
+    | mkMVec LOAD      Lpc LI [REG; DATA _ _ _; REG] => rvec_next        Lpc LI
+    | mkMVec STORE     Lpc LI [REG; REG; DATA c I W] => rvec_store c I W Lpc LI
+    | mkMVec JUMP      Lpc LI [REG]                  => rvec_jump        Lpc LI
+    | mkMVec BNZ       Lpc LI [REG]                  => rvec_next        Lpc LI
+    | mkMVec JAL       Lpc LI [REG; REG]             => rvec_jump        Lpc LI
+    | mkMVec SERVICE   _   _  []                     => Some (mkRVec REG REG)
+    | mkMVec _         _   _  _                      => None
   end.
 
 End WithVectors.
@@ -215,13 +219,12 @@ Fixpoint retag_set (ok : word t -> list (word t) -> list (word t) -> bool)
                    : option (memory * sfi_internal) :=
   match ps with
     | []       => Some (M,si)
-    | p :: ps' => do! x @ L          <-  get M p;
-                  do! x @ DATA c I W <-  get M p;
+    | p :: ps' => do! x @ DATA c I W <-  get M p;
                   do! guard (ok c I W);
                   do! DATA _ I' W'   <-! retag c I W;
                   do! si'            <-  register_set I' si;
-                  do! si''           <-  register_set W' si;
-                  do! M'             <-  upd M p (x @ L);
+                  do! si''           <-  register_set W' si';
+                  do! M'             <-  upd M p (x @ (DATA c I' W'));
                   retag_set ok retag ps' M' si''
   end.
 
@@ -248,7 +251,7 @@ Definition isolate (s : Symbolic.state t) : option (Symbolic.state t) :=
       do! S'       <- isolate_create_set (@val _ _) M pS;
       do! (MS,siS) <- retag_set (fun c'' _ W => (c == c'') || set_elem c W)
                                 (fun c'' I W => DATA c'' I (insert_unique c' W))
-                                J' MJ siJ;
+                                S' MJ siJ;
 
       Some (Symbolic.State MS R ((pc + 1)%w @ (PC INTERNAL c)) siS)
     | _ => None
@@ -298,20 +301,486 @@ Definition interned_tag (ids : list (list (word t) * word t))
   match L with
     | DATA _ I W => is_some (assoc_list_lookup ids (eq_op I)) &&
                     is_some (assoc_list_lookup ids (eq_op W))
-    | _ => true (* or false *)
+    | _ => false (* or true *)
   end.
 
-(* good_internal & interned_tag -> all lists are sets *)
+Definition good_memory_tag (ids : list (list (word t) * word t))
+                           (M : Symbolic.memory t)
+                           (p : word t) : bool :=
+  match get M p with
+    | Some (_ @ (DATA _ I W)) =>
+      is_some (assoc_list_lookup ids (eq_op I)) &&
+      is_some (assoc_list_lookup ids (eq_op W))
+    | Some (_ @ _)            => false
+    | None                    => true
+  end.
+
+Definition good_register_tag (R : Symbolic.registers t) (r : reg t) : bool :=
+  match get R r with
+    | Some (_ @ REG) => true
+    | Some (_ @ _)   => false
+    | None           => true
+  end.
+
+Definition good_pc_tag (pc : atom (word t) stag) : bool :=
+  match pc with
+    | _ @ (PC _ _) => true
+    | _ @ _        => false
+  end.
 
 Definition good_tags (s : Symbolic.state t) : Prop :=
-  let: Symbolic.State M R pc si := s in
-  (forall p v, get M p = Some v -> stag_is_DATA (common.tag v) &&
-                                   interned_tag (set_ids si) (common.tag v)) /\
-  (forall r v, get R r = Some v -> stag_is_REG  (common.tag v)) /\
-  stag_is_PC (common.tag pc).
+  let: Symbolic.State M R pc (Internal next ids) := s in
+  (forall p, good_memory_tag   ids M p) /\
+  (forall r, good_register_tag     R r) /\
+  good_pc_tag pc.
 
 Definition good_state (s : Symbolic.state t) : Prop :=
   good_tags s /\ good_internal (Symbolic.internal s).  
+
+(* Implied by the others *)
+Definition memory_has_sets (M : memory) (p : word t) : bool :=
+  match get M p with
+    | Some (_ @ (DATA _ I W)) => is_set I && is_set W
+    | Some (_ @ _)            => false
+    | None                    => true
+  end.
+
+Generalizable All Variables.
+
+Ltac undo1 hyp var :=
+  let def_var := fresh "def_" var in
+  match type of hyp with
+    | (do! _ <- ?GET; _) = Some _ =>
+      destruct GET as [var|] eqn:def_var
+    | (do! guard ?COND; _) = Some _ =>
+      destruct COND eqn:var
+  end; simpl in hyp; [|discriminate].
+
+Ltac undo2 hyp v1 v2 :=
+  let GET := match type of hyp with
+               | (do! (_,_) <- ?GET; _) = Some _ => GET
+               | (do! _ @ _ <- ?GET; _) = Some _ => GET
+             end
+  in let def_v1_v2 := fresh "def_" v1 "_" v2 in
+     destruct GET as [[v1 v2]|] eqn:def_v1_v2;
+     simpl in hyp; [|discriminate].
+
+Ltac undoDATA hyp x c I W :=
+  let xcIW := fresh "xcIW" in
+  undo1 hyp xcIW; destruct xcIW as [x [|c I W|]];
+  [discriminate | simpl in hyp | discriminate].
+
+Corollary assoc_list_lookup_some_eq : forall (K : eqType) V (kvs : list (K * V))
+                                             k v,
+  assoc_list_lookup kvs (eq_op k) = Some v ->
+  In (k,v) kvs.
+Proof.
+  intros K V kvs k v ASSOC; apply assoc_list_lookup_some in ASSOC.
+  case ASSOC => [k' [/eqP<- IN]]; exact IN.
+Qed.
+
+Corollary in_assoc_list_lookup_eq : forall (K : eqType) V (kvs : list (K * V))
+                                           k v,
+  In (k,v) kvs ->
+  exists v', assoc_list_lookup kvs (eq_op k) = Some v'.
+Proof.
+  intros K V kvs k v IN; eapply in_assoc_list_lookup in IN;
+    [eassumption | apply eq_refl].
+Qed.
+
+Lemma good_internal_and_memory__memory_has_sets : forall si M p,
+  good_internal si ->
+  good_memory_tag (set_ids si) M p ->
+  memory_has_sets M p.
+Proof.
+  clear S I.
+  unfold good_memory_tag, memory_has_sets; intros si M p GOOD MEM.
+  set GET := get M p in MEM *; destruct GET as [[x [|c I W|]]|]; auto.
+  destruct si as [next ids]; simpl in *.
+  assert (SET : forall X, is_some (assoc_list_lookup ids (eq_op X)) ->
+                          is_set X). {
+    clear MEM; intros X SOME.
+    destruct (assoc_list_lookup _ _) as [id|] eqn:ASSOC; simpl in *; auto.
+    apply assoc_list_lookup_some_eq in ASSOC.
+    move/forallb_forall in GOOD; apply GOOD in ASSOC.
+    by move: ASSOC => /andP [].
+  }
+  move: MEM => /andP [IN_I IN_W]; apply/andP; auto.
+Qed.
+
+Corollary good_state__good_memory : forall s,
+  good_state s ->
+  forall p, memory_has_sets (Symbolic.mem s) p.
+Proof.
+  unfold good_state,good_tags;
+    move=> [M R pc [next ids]] [[MEM [REG PC]] INT] p.
+  eapply good_internal_and_memory__memory_has_sets; eauto.
+Qed.
+
+Lemma fresh_preserves_good : forall si si' fid,
+  fresh si = Some (fid,si') ->
+  good_internal si ->
+  good_internal si'.
+Proof.
+  intros [next ids] [next' ids'] fid FRESH; simpl in *.
+  destruct (next == max_word) eqn:BOUND; [discriminate|].
+  move=> /eqP in BOUND.
+  inversion FRESH; subst; clear FRESH.
+  apply forallb_impl.
+  move=> [set id] /andP [SET LT]; andb_true_split; auto.
+  eapply ltb_trans; [exact LT | apply lebw_succ with max_word].
+  generalize (lew_max fid) => /le_iff_lt_or_eq [] //.
+Qed.
+
+Lemma register_set_preserves_good : forall si si' X,
+  is_set X ->
+  register_set X si = Some si' ->
+  good_internal si ->
+  good_internal si'.
+Proof.
+  clear S I.
+  move=> [next ids] [next' ids'] /= X SET REG GOOD.
+  destruct (assoc_list_lookup _ _) eqn:LOOKUP.
+  - inversion REG; subst; exact GOOD.
+  - destruct (next == max_word) eqn:MAX; simpl in REG; inversion REG; subst.
+    simpl; andb_true_split; auto.
+    + apply lebw_succ with max_word.
+      generalize (lew_max next) => MAX'; apply le__lt_or_eq in MAX'.
+      destruct MAX'; [assumption | subst; rewrite eq_refl in MAX; discriminate].
+    + eapply forallb_impl; [|apply GOOD]; cbv beta.
+      move=> [set id] /andP [SET' LT]; apply /andP; split; auto.
+      eapply ltb_trans; [apply LT | apply lebw_succ with max_word].
+      generalize (lew_max next) => MAX'; apply le__lt_or_eq in MAX'.
+      destruct MAX'; [assumption | subst; rewrite eq_refl in MAX; discriminate].
+Qed.
+
+Lemma retag_set_preserves_good : forall si si' ok retag ps M M',
+  (forall osi c I W,
+     good_internal osi ->
+     is_some (assoc_list_lookup (set_ids osi) (eq_op I)) ->
+     is_some (assoc_list_lookup (set_ids osi) (eq_op W)) ->
+     match retag c I W with
+       | DATA _ I' W' =>
+         match bind (register_set W') (register_set I' osi) with
+           | Some osi' =>
+             is_set I' && is_set W' &&
+             is_some (assoc_list_lookup (set_ids osi') (eq_op I')) &&
+             is_some (assoc_list_lookup (set_ids osi') (eq_op W')) /\
+             forall X,
+               is_some (assoc_list_lookup (set_ids osi)  (eq_op X)) ->
+               is_some (assoc_list_lookup (set_ids osi') (eq_op X))
+           | None => True
+         end
+       | _ => False
+     end) ->
+  retag_set ok retag ps M si = Some (M',si') ->
+  (forall p, good_memory_tag (set_ids si) M p) ->
+  good_internal si ->
+  (forall p, good_memory_tag (set_ids si') M' p) /\ good_internal si'.
+Proof.
+  clear S I.
+  intros si si' ok retag ps M M' RETAG RETAG_SET; simpl.
+  move: si si' M M' RETAG_SET; induction ps as [|p ps];
+    move=> /= si si' M M' RETAG_SET.
+  - by inversion RETAG_SET; subst.
+  - idtac;
+      undoDATA RETAG_SET x c I' W; rename I' into I;
+      undo1 RETAG_SET OK;
+      destruct (retag c I W) as [|c' I' W'|] eqn:def_c'_I'_W'; try discriminate;
+      undo1 RETAG_SET si1; undo1 RETAG_SET si2; undo1 RETAG_SET M2.
+    intros MEM GOOD.
+    unfold good_memory_tag in *.
+    move: (MEM p); rewrite def_xcIW; move=> /andP [OK_I OK_W].
+    specialize (RETAG si c I W GOOD OK_I OK_W);
+      rewrite def_c'_I'_W' def_si1 /= def_si2 in RETAG;
+      repeat rewrite <-Bool.andb_assoc in RETAG;
+      case: RETAG => [/and4P[SET_I' SET_W' OK_I' OK_W'] PRESERVE].
+    eapply IHps; try eassumption.
+    + intros p'; destruct (p == p') eqn:EQ_p_p'; move/eqP in EQ_p_p'.
+      * subst p'.
+        apply get_upd_eq in def_M2; [rewrite def_M2 | exact sma].
+        by apply/andP.
+      * apply get_upd_neq with (key' := p') in def_M2; auto.
+        rewrite def_M2; specialize MEM with p'.
+        set GET_M_p' := get M p' in MEM *;
+          destruct GET_M_p' as [[? [|c'' I'' W''|]]|]; auto.
+        move/andP in MEM; apply/andP; split; apply PRESERVE; tauto.
+    + do 2 (
+        eapply register_set_preserves_good; [|eassumption|]; [eassumption|]
+      ); assumption.
+Qed.
+
+Theorem isolate_good : forall s s',
+  isolate s = Some s' ->
+  good_state s ->
+  good_state s'.
+Proof.
+  clear S I.
+  intros [M R [pc [S c| |]] si] s' ISOLATE GOOD;
+    simpl in *; try discriminate.
+  let DO2 := undo2 ISOLATE in let DO1 := undo1 ISOLATE
+  in DO2 c' si'; DO2 pA LA; DO2 pJ LJ; DO2 pS LS;
+     DO1 A'; DO1 NONEMPTY_A'; DO2 MA siA;
+     DO1 J'; DO2 MJ siJ;
+     DO1 S'; DO2 MS siS;
+     inversion ISOLATE; subst; clear ISOLATE; simpl.
+  rewrite /good_state /= in GOOD; destruct GOOD as [TAGS INT].
+  assert (GOOD_si' : good_internal si') by eauto 2 using fresh_preserves_good.
+  assert (GOOD_MA_siA : (forall p, good_memory_tag (set_ids siA) MA p) /\
+                        good_internal siA). {
+    apply retag_set_preserves_good in def_MA_siA; auto.
+    - intros osi _ I W OGOOD OK_I OK_W;
+        destruct (register_set I osi)  as [osi'|]  eqn:REG; simpl; auto;
+        destruct (register_set W osi') as [osi''|] eqn:REG'; auto.
+      unfold register_set in *;
+        destruct osi as [onext oids], osi' as [onext' oids']; simpl in *.
+      destruct (assoc_list_lookup oids (eq_op I)) eqn:ASSOC_I;
+        auto; simpl in *.
+      inversion REG; subst; simpl in *.
+      destruct (assoc_list_lookup oids' (eq_op W)) eqn:ASSOC_W;
+        auto; simpl in *.
+      inversion REG'; subst; simpl in *.
+      rewrite ASSOC_I ASSOC_W; simpl; do ! rewrite andbT.
+      split; auto.
+      hnf in OGOOD; rewrite ->forallb_forall in OGOOD;
+        apply assoc_list_lookup_some_eq, OGOOD in ASSOC_W;
+        apply assoc_list_lookup_some_eq, OGOOD in ASSOC_I;
+        move: ASSOC_W ASSOC_I => /andP[SET_W _] /andP[SET_I _].
+      by apply/andP.
+    - destruct si as [next ids], TAGS as [MEM [REG _]]; simpl in def_c'_si'.
+      destruct (next == max_word); [discriminate|].
+      inversion def_c'_si'; subst; simpl in *; apply MEM.
+  }
+  assert (GOOD_MJ_siJ : (forall p, good_memory_tag (set_ids siJ) MJ p) /\
+                        good_internal siJ). {
+    apply retag_set_preserves_good in def_MJ_siJ; try tauto.
+    intros osi _ I W OGOOD OK_I OK_W;
+      destruct (register_set (insert_unique c' I) osi)  as [osi'|] eqn:REG;
+      simpl; auto;
+      destruct (register_set W osi') as [osi''|] eqn:REG'; auto.
+    unfold register_set in *;
+      destruct osi as [onext oids], osi' as [onext' oids']; simpl in *.
+    hnf in OGOOD; rewrite ->forallb_forall in OGOOD.
+    destruct (assoc_list_lookup oids (eq_op I)) eqn:ASSOC_I; auto.
+    destruct (assoc_list_lookup oids (eq_op (insert_unique c' I)))
+             eqn:ASSOC_I';
+      auto; simpl in *.
+    - inversion REG; subst; simpl in *.
+      destruct (assoc_list_lookup oids' (eq_op W)) eqn:ASSOC_W;
+        auto; simpl in *.
+      inversion REG'; subst; simpl in *.
+      rewrite ASSOC_I' ASSOC_W; simpl; do ! rewrite andbT.
+      split; auto;
+        apply assoc_list_lookup_some_eq, OGOOD in ASSOC_W;
+        apply assoc_list_lookup_some_eq, OGOOD in ASSOC_I';
+        move: ASSOC_W ASSOC_I' => /andP[SET_W _] /andP[SET_I' _].
+      by apply/andP.
+    - destruct (onext == max_word); [discriminate|]; simpl in REG.
+      inversion REG; subst; simpl in *.
+      destruct (assoc_list_lookup oids (eq_op W)) eqn:ASSOC_W; auto;
+        simpl in *.
+      destruct (W == insert_unique c' I) eqn:EQ_W; [move: EQ_W => /eqP->|];
+        inversion REG'; subst; simpl in *.
+      + rewrite eq_refl; simpl in *.
+        do ! rewrite andbT; rewrite Bool.andb_diag.
+        split; [|intros X SOME; destruct (X == _); auto].
+        apply insert_unique_preserves_set_true.
+        apply assoc_list_lookup_some_eq,OGOOD in ASSOC_I.
+        by move: ASSOC_I => /andP[].
+      + rewrite eq_refl EQ_W ASSOC_W; simpl; do ! rewrite andbT.
+        split; [|intros X SOME; destruct (X == _); auto].
+        idtac;
+          apply assoc_list_lookup_some_eq,OGOOD in ASSOC_I;
+          apply assoc_list_lookup_some_eq,OGOOD in ASSOC_W.
+        move: ASSOC_W ASSOC_I => /andP[SET_W _] /andP[SET_I _].
+        apply/andP; auto.
+  }
+  assert (GOOD_MS_siS : (forall p, good_memory_tag (set_ids siS) MS p) /\
+                        good_internal siS). {
+    apply retag_set_preserves_good in def_MS_siS; try tauto.
+    intros osi _ I W OGOOD OK_I OK_W;
+      destruct (register_set I osi)  as [osi'|] eqn:REG; simpl; auto;
+      destruct (register_set (insert_unique c' W) osi') as [osi''|] eqn:REG';
+      auto.
+    unfold register_set in *;
+      destruct osi as [onext oids], osi' as [onext' oids']; simpl in *.
+    hnf in OGOOD; rewrite ->forallb_forall in OGOOD.
+    destruct (assoc_list_lookup oids (eq_op W)) eqn:ASSOC_W; auto.
+    destruct (assoc_list_lookup oids (eq_op I)) eqn:ASSOC_I; auto.
+    inversion REG; subst; simpl in *.
+    destruct (assoc_list_lookup oids' (eq_op (insert_unique c' W)))
+             eqn:ASSOC_W'.
+    - inversion REG'; subst; simpl in *.
+      rewrite ASSOC_I ASSOC_W'; simpl; do ! rewrite andbT.
+      split; auto;
+        apply assoc_list_lookup_some_eq, OGOOD in ASSOC_I;
+        apply assoc_list_lookup_some_eq, OGOOD in ASSOC_W';
+        move: ASSOC_I ASSOC_W' => /andP[SET_I _] /andP[SET_W' _].
+      by apply/andP.
+    - destruct (onext' == max_word); [discriminate|]; simpl in REG'.
+      inversion REG'; subst; simpl in *.
+      destruct (I == insert_unique c' W) eqn:EQ_I; [move: EQ_I => /eqP->|].
+      + rewrite eq_refl; simpl in *.
+        do ! rewrite andbT; rewrite Bool.andb_diag.
+        split; [|intros X SOME; destruct (X == _); auto].
+        apply insert_unique_preserves_set_true.
+        apply assoc_list_lookup_some_eq,OGOOD in ASSOC_W.
+        by move: ASSOC_W => /andP[].
+      + rewrite eq_refl ASSOC_I; simpl; do ! rewrite andbT.
+        split; [|intros X SOME; destruct (X == _); auto].
+        idtac;
+          apply assoc_list_lookup_some_eq,OGOOD in ASSOC_I;
+          apply assoc_list_lookup_some_eq,OGOOD in ASSOC_W.
+        move: ASSOC_W ASSOC_I => /andP[SET_W _] /andP[SET_I _].
+        apply/andP; auto.
+  }
+  destruct si as [next ids], siS as [nextS idsS]; rewrite /good_state /=; tauto.
+Qed.
+
+Theorem add_to_jump_targets_good : forall s s',
+  add_to_jump_targets s = Some s' ->
+  good_state s ->
+  good_state s'.
+Proof.
+  clear S I.
+  intros [M R [pc [S c| |]] si] s' ADD GOOD; try discriminate; simpl in *.
+  undo2 ADD p Lp; undo2 ADD x Lx; destruct Lx as [|c' I W|]; try discriminate;
+    undo1 ADD si'; undo1 ADD M'.
+  inversion ADD; subst; simpl in *.
+  destruct si as [next ids].
+  rewrite /good_state /= in GOOD; destruct GOOD as [[MEM [REG _]] INT].
+  assert (SET_I : is_set I). {
+    specialize MEM with p; unfold good_memory_tag in MEM;
+      rewrite def_x_Lx in MEM; move: MEM => /andP [OK_I OK_W].
+    unfold is_true in INT; rewrite ->forallb_forall in INT.
+    destruct (assoc_list_lookup ids (eq_op I)) eqn:ASSOC_I; auto.
+    apply assoc_list_lookup_some_eq,INT in ASSOC_I.
+    by move: ASSOC_I => /andP [].
+  }
+  assert (INT' : good_internal si') by
+    (apply register_set_preserves_good in def_si'; auto).
+  rewrite /good_state /=.
+  destruct si' as [next' ids']; repeat split; try tauto.
+  simpl in def_si'.
+  intros p'; specialize MEM with p'; unfold good_memory_tag in *.
+  destruct (p == p') eqn:EQ_P; move/eqP in EQ_P; [subst p'|].
+  - apply get_upd_eq in def_M'; [rewrite def_M' | exact sma].
+    rewrite def_x_Lx in MEM.
+    move: MEM => /andP [OK_I OK_W]; apply/andP.
+    destruct (assoc_list_lookup ids (eq_op (insert_unique c I))) eqn:ASSOC_I'.
+    + by inversion def_si'; subst; rewrite ASSOC_I'.
+    + destruct (next == max_word); [discriminate|]; simpl in def_si';
+        inversion def_si'; subst; simpl in *.
+      by rewrite eq_refl; destruct (W == insert_unique c I).
+  - apply get_upd_neq with (key' := p') in def_M'; auto; rewrite def_M'.
+    set GET_M_p' := get M p' in MEM *;
+      destruct GET_M_p' as [[? [|c'' I'' W''|]]|]; auto.
+    destruct (assoc_list_lookup ids (eq_op (insert_unique c I))) eqn:ASSOC_I'.
+    + by inversion def_si'; subst.
+    + destruct (next == max_word); [discriminate|]; simpl in def_si';
+        inversion def_si'; subst; simpl in *.
+      move: MEM => /andP [OK_I'' OK_W''].
+      by apply/andP; destruct (I'' == _), (W'' == _).
+Qed.
+
+Theorem add_to_shared_memory_good : forall s s',
+  add_to_shared_memory s = Some s' ->
+  good_state s ->
+  good_state s'.
+Proof.
+  clear S I.
+  intros [M R [pc [S c| |]] si] s' ADD GOOD; try discriminate; simpl in *.
+  undo2 ADD p Lp; undo2 ADD x Lx; destruct Lx as [|c' I W|]; try discriminate;
+    undo1 ADD si'; undo1 ADD M'.
+  inversion ADD; subst; simpl in *.
+  destruct si as [next ids].
+  rewrite /good_state /= in GOOD; destruct GOOD as [[MEM [REG _]] INT].
+  assert (SET_I : is_set W). {
+    specialize MEM with p; unfold good_memory_tag in MEM;
+      rewrite def_x_Lx in MEM; move: MEM => /andP [OK_I OK_W].
+    unfold is_true in INT; rewrite ->forallb_forall in INT.
+    destruct (assoc_list_lookup ids (eq_op W)) eqn:ASSOC_W; auto.
+    apply assoc_list_lookup_some_eq,INT in ASSOC_W.
+    by move: ASSOC_W => /andP [].
+  }
+  assert (INT' : good_internal si') by
+    (apply register_set_preserves_good in def_si'; auto).
+  rewrite /good_state /=.
+  destruct si' as [next' ids']; repeat split; try tauto.
+  simpl in def_si'.
+  intros p'; specialize MEM with p'; unfold good_memory_tag in *.
+  destruct (p == p') eqn:EQ_P; move/eqP in EQ_P; [subst p'|].
+  - apply get_upd_eq in def_M'; [rewrite def_M' | exact sma].
+    rewrite def_x_Lx in MEM.
+    move: MEM => /andP [OK_I OK_W]; apply/andP.
+    destruct (assoc_list_lookup ids (eq_op (insert_unique c W))) eqn:ASSOC_W'.
+    + by inversion def_si'; subst; rewrite ASSOC_W'.
+    + destruct (next == max_word); [discriminate|]; simpl in def_si';
+        inversion def_si'; subst; simpl in *.
+      by rewrite eq_refl; destruct (I == insert_unique c W).
+  - apply get_upd_neq with (key' := p') in def_M'; auto; rewrite def_M'.
+    set GET_M_p' := get M p' in MEM *;
+      destruct GET_M_p' as [[? [|c'' I'' W''|]]|]; auto.
+    destruct (assoc_list_lookup ids (eq_op (insert_unique c W))) eqn:ASSOC_W'.
+    + by inversion def_si'; subst.
+    + destruct (next == max_word); [discriminate|]; simpl in def_si';
+        inversion def_si'; subst; simpl in *.
+      move: MEM => /andP [OK_I'' OK_W''].
+      by apply/andP; destruct (I'' == _), (W'' == _).
+Qed.
+
+Theorem good_state_preserved : forall `(STEP : step s s'),
+  good_state s ->
+  good_state s'.
+Proof.
+  clear S I.
+  intros s s' STEP GOOD; destruct STEP;
+    unfold Symbolic.next_state_reg, Symbolic.next_state_pc,
+           Symbolic.next_state_reg_and_pc, Symbolic.next_state in *;
+    simpl in *;
+    unfold rvec_next, rvec_jump, rvec_store, rvec_simple, rvec_step in *;
+    repeat match goal with
+      | NEXT : (do! _ <- ?m; _) = Some _ |- _ =>
+        destruct m eqn:?; simpl in NEXT; [|discriminate]
+      | TAG  : match ?t with _ => _ end = Some _ |- _ =>
+        destruct t; try discriminate
+      | EQN  : Some _ = Some _ |- _ =>
+        inversion EQN; subst; simpl; auto; clear EQN
+    end;
+    try (
+      destruct int as [next ids], GOOD as [[MEM [REG PC]] INT];
+      repeat split; try tauto;
+      let k' := fresh "k'" in
+      intros k';
+      match goal with
+        | UPD : upd _ ?k _ = Some _ |- appcontext[?good_fn _] =>
+          unfold good_fn;
+          destruct (k' == k) eqn:EQ; move/eqP in EQ;
+          [ subst; apply get_upd_eq in UPD
+          | apply get_upd_neq with (key' := k') in UPD ];
+          auto; rewrite UPD;
+          [ auto
+          | first [apply MEM | apply REG] ]
+      end);
+    simpl in *;
+    try match type of CALL with
+      | ?t =>
+        match t with
+          | Symbolic.run_syscall (Symbolic.Syscall _ _ ?fn) _ = _ =>
+            replace t with (fn (Symbolic.State mem reg pc@tpc int) = Some s')
+              in * by reflexivity
+        end
+    end.
+  - (* store *)
+    unfold is_true in INT; rewrite ->forallb_forall in INT.
+    by specialize MEM with w1; rewrite /good_memory_tag OLD in MEM.
+  - (* isolate *)
+    apply isolate_good in CALL; assumption.
+  - (* add_to_jump_targets *)
+    apply add_to_jump_targets_good in CALL; assumption.
+  - (* add_to_shared_memory *)
+    apply add_to_shared_memory_good in CALL; assumption.
+Qed.
 
 End WithClasses.
 
